$$
\cos nx = \frac{1}{2} \, (e^{nxi} + e^{-nxi}) \;,\;\;
\sin nx = \frac{1}{2} \, (e^{nxi} - e^{-nxi})
$$

$\implies$

$$
a_0 + \sum\limits_{n=1}^{+\infty}
\left(
	a_n \cos nx + b_n \sin nx
\right)
=
\sum\limits_{n=-\infty}^{+\infty} c_n e^{inx}
$$

где

$$
c_0 = a_0 \;,\;\;
c_n = \frac{1}{2}(a_n-b_ni) \;,\;\;
c_{-n} = \frac{1}{2}(a_n+b_ni) \;,\;\;
n \in \mathbb{N}
$$

---

Если 
$$
f(x) = a_0 + \sum\limits_{n=1}^{+\infty}
\left(
	a_n \cos nx + b_n \sin nx
\right)
$$
то
$$
c_n =
\frac{1}{2\pi}
\int\limits_{-\pi}^{\pi}
	f(x) e^{-inx} \; dx
$$